New versions of generated files

examples/theorem_generation.v
@@ -9,25 +9,27 @@ Require Import listPairSml.
 Require Import notationsSml.
 From Equations Require Import Equations.
 
+Generalizable All Variables.
+
 Equations posAdd (x1: (Z * Z)%type): Z :=
   posAdd (x, y) := (x + y).
 
-Theorem posAdd_THM: forall ' ((x, y), b), (((posAdd (x, y) = b) /\ ((((x > 0) && (y > 0))) = true)) -> ((((b > x) && (b > y))) = true)).
+Theorem posAdd_THM: forall x y b, posAdd (x, y) = b /\ ((x > 0) && (y > 0)) = true -> ((b > x) && (b > y)) = true.
 Admitted.
 
 Equations negAdd (x1: Z) (x2: Z): Z :=
   negAdd x y := (x + y).
 
-Theorem negAdd_THM: forall ' (x, y, b), (((negAdd x y = b) /\ ((((x > 0) && (y > 0))) = true)) -> ((((b > x) && (b > y))) = true)).
+Theorem negAdd_THM: forall `(x:Z) `(y:Z) `(b:Z), negAdd x y = b /\ ((x < 0) && (y < 0)) = true -> ((b < x) && (b < y)) = true.
 Admitted.
 
-Equations trueLen (x1: (@list Z)): Z :=
+Equations trueLen (x1: @list Z): Z :=
   trueLen [] := 0;
-  trueLen (a :: l) := (1 + ((trueLen l))).
+  trueLen (a :: l) := (1 + (trueLen l)).
 
-Equations len {_'13565: Type} (x1: (@list _'13565)): Z :=
+Equations len `(x1: @list _'14129): Z :=
   len [] := 0;
-  len (x :: l') := (1 + ((len l'))).
+  len (x :: l') := (1 + (len l')).
 
-Theorem len_THM: forall ' (l, result), (((len l = result) /\ ((((((List.length l))) >= 0)) = true)) -> (((result = (((trueLen l))))) = true)).
+Theorem len_THM: forall `(l:@list Z) `(result:Z), len l = result /\ ((((List.length l)) >= 0)) = true -> ((result = ((trueLen l)))) = true.
 Admitted.
