examples/functor.v
@@ -9,26 +9,28 @@ Require Import listPairSml.
 Require Import notationsSml.
 From Equations Require Import Equations.
 
+Generalizable All Variables.
+
 Module Type KEY.
 
 Parameter t : Type.
 
-Parameter compare : ((t * t) % type -> comparison).
+Parameter compare : (t * t)%type -> comparison.
 End KEY.
 
 Module Type DICT.
 
 Parameter key : Type.
 
-Definition entry {_a : Type} := (key * _a) % type.
+Definition entry {_a : Type} := (key * _a)%type.
 
-Parameter dict : (Type -> Type).
+Parameter dict : Type -> Type.
 
-Parameter empty : (forall  {_a : Type} , (@ dict _a)).
+Parameter empty : forall  {_a : Type}, @dict _a.
 
-Parameter lookup : (forall  {_a : Type} , ((key * (@ dict _a)) % type -> (@ option _a))).
+Parameter lookup : forall  {_a : Type}, (key * @dict _a)%type -> @option _a.
 
-Parameter insert : (forall  {_a : Type} , (((@ entry _a) * (@ dict _a)) % type -> (@ dict _a))).
+Parameter insert : forall  {_a : Type}, (@entry _a * @dict _a)%type -> @dict _a.
 End DICT.
 
 Module IntKey : KEY with 
@@ -53,33 +55,33 @@ Module K := Key.
 
 Definition key := K.t.
 
-Definition entry {_a : Type} := (key * _a) % type.
+Definition entry {_a : Type} := (key * _a)%type.
 
-Definition dict {_a : Type} := (key -> (@ option _a)).
+Definition dict {_a : Type} := key -> @option _a.
 
-Equations empty {_'13510: Type} (x1: key): (@ option _'13510) :=
+Equations empty (x1: key): @option _'13533 :=
   empty k := None.
 
-Equations lookup {_a: Type} (x1: (key * (key -> (@ option _a)))): (@ option _a) :=
-  lookup (k, f) := ((f k)).
+Equations lookup `(x1: (key * key -> @option _a)%type): @option _a :=
+  lookup (k, f) := (f k).
 
-Equations insert {_a: Type} (x1: ((@ entry _a) * (key -> (@ option _a)))): (key -> (@ option _a)) :=
-  insert ((k, v), f) := (fun  _id13577 => 
-  match _id13577 with
+Equations insert `(x1: (@entry _a * key -> @option _a)%type): key -> @option _a :=
+  insert ((k, v), f) := (fun _id13607 => 
+  match _id13607 with
   | k' => 
-  match ((K.compare (k, k'))) with
-  | Eq => ((Some v))  
-  | _ => ((f k'))
+  match (K.compare (k, k')) with
+  | Eq => (Some v)  
+  | _ => (f k')
   end
   end).
 End Dict.
 
 Module IntDict := !Dict IntKey.
 
-Definition id1 := ((IntDict.insert ((42, "answer"), IntDict.empty))).
+Definition id1 := (IntDict.insert ((42, "answer"), IntDict.empty)).
 
 Definition a := 
-  match ((IntDict.lookup (42, id1))) with
+  match (IntDict.lookup (42, id1)) with
   (Some a) => a
   | _ => patternFailure
   end.
