examples/non_terminating.v
@@ -9,24 +9,27 @@ Require Import listPairSml.
 Require Import notationsSml.
 From Equations Require Import Equations.
 
-Equations loop1 {_'13691: Type} (x1: Z): _'13691 :=
-  loop1 x := ((loop1 (x + 1))).
+Generalizable All Variables.
 
-Equations loop2 {_'13701: Type} (x1: Z): _'13701 :=
-  loop2 x := ((loop2 (x - 1))).
+Equations loop1 (x1: Z): _'13722 :=
+  loop1 x := (loop1 ((x + 1))).
 
-Equations loop3 {_'13717: Type} {_'13718: Type} (x1: (@ list _'13717)) {H: (exists  y1  y2 , eq (x1) (y1 :: y2))}: _'13718 :=
-  loop3 (x :: l) := ((loop3 (l @ [x])));
+Equations loop2 (x1: Z): _'13732 :=
+  loop2 x := (loop2 ((x - 1))).
+
+Equations loop3 `(x1: @list _'13748) {H: exists y1 y2 , eq (x1) (y1 :: y2)}: _'13749 :=
+  loop3 (x :: l) := (@loop3 ((l @ [x])) _);
   loop3 _ := _.
+Admit Obligations.
 
 Equations fact (x1: Z): Z :=
   fact 0 := 1;
-  fact n := n * ((fact (n - 1))).
+  fact n := (n * (fact ((n - 1)))).
 
-Equations collatz (x1: Z): (@ list Z) :=
+Equations collatz (x1: Z): @list Z :=
   collatz 1 := [1];
-  collatz n := n :: (
-  match n mod 2 with
-  | 0 => ((collatz (n div 2)))  
-  | _ => ((collatz (3 * n + 1)))
-  end).
+  collatz n := (n :: (
+  match (n mod 2) with
+  | 0 => (collatz ((n div 2)))  
+  | _ => (collatz (((3 * n) + 1)))
+  end)).
