examples/terminating.v
@@ -9,42 +9,45 @@ Require Import listPairSml.
 Require Import notationsSml.
 From Equations Require Import Equations.
 
+Generalizable All Variables.
+
 Inductive tree  : Type := 
-  | Leaf : (Z -> (@ tree ))  
-  | Node : ((tree * tree) % type -> (@ tree )).
+  | Leaf : Z -> @tree   
+  | Node : (tree * tree)%type -> @tree .
 
-Equations treeListSum (x1: (@ list tree)): Z :=
+Equations treeListSum (x1: @list tree): Z :=
   treeListSum [] := 0;
-  treeListSum ((Leaf y) :: xs) := y + ((treeListSum xs));
-  treeListSum ((Node (l, r)) :: xs) := ((treeListSum (l :: r :: xs))).
+  treeListSum ((Leaf y) :: xs) := (y + (treeListSum xs));
+  treeListSum ((Node (l, r)) :: xs) := (treeListSum ((l :: (r :: xs)))).
 
-Equations remove (x1: (Z * (@ list Z))) {H: (exists  y1  y2  y3 , eq (x1) ((y1, y2 :: y3)))}: (@ list Z) :=
-  remove (x, (y :: l)) := if x = y then l else y :: ((remove (x, l)));
+Equations remove (x1: (Z * @list Z)%type) {H: exists y1 y2 y3 , eq (x1) ((y1, y2 :: y3))}: @list Z :=
+  remove (x, (y :: l)) := if (x = y) then l else (y :: (@remove (x, l) _));
   remove _ := _.
+Admit Obligations.
 
-Equations isPermutation (x1: ((@ list Z) * (@ list Z))): bool :=
+Equations isPermutation (x1: (@list Z * @list Z)%type): bool :=
   isPermutation ([], []) := true;
-  isPermutation ((x :: l), l') := (((((List.existsb (fun  _id13935 => 
-  match _id13935 with
-  | e => e = x
-  end))) l'))) && ((isPermutation (l, ((remove (x, l'))))));
+  isPermutation ((x :: l), l') := (((List.existsb (fun _id13974 => 
+  match _id13974 with
+  | e => (e = x)
+  end)) l')) && (isPermutation (l, (@remove (x, l') _)));
   isPermutation _ := false.
 
-Equations permutations {_''13930: Type} (x1: (@ list _''13930)): (@ list (@ list _''13930)) :=
+Equations permutations `(x1: @list _''13962): @list @list _''13962 :=
   permutations l := 
   match l with
   | [] => []  
   | [x] => [[x]]  
-  | _ => ((((((List.foldl (fun  _id13936 => 
-  match _id13936 with
+  | _ => (((List.foldl (fun _id13975 => 
+  match _id13975 with
   | (x, acc) => 
-  let l_no_x := ((((List.filter (fun  _id13937 => 
-  match _id13937 with
-  | e => e <> x
-  end))) l)) in 
-  let ps := ((permutations l_no_x)) in acc @ ((((List.map (fun  _id13938 => 
-  match _id13938 with
-  | p => x :: p
-  end))) ps))
-  end))) [])) l))
+  let l_no_x := ((List.filter (fun _id13976 => 
+  match _id13976 with
+  | e => (e <> x)
+  end)) l) in 
+  let ps := (permutations l_no_x) in (acc @ ((List.map (fun _id13977 => 
+  match _id13977 with
+  | p => (x :: p)
+  end)) ps))
+  end)) []) l)
   end.
